finish proving first condition of safe predicate

GCSL.v
@@ -25,16 +25,28 @@ Definition bdiv_g (gs : g_state nblk ntrd) :=
   exists bid : Fin.t nblk, 
     Bdiv.bdiv ((blks gs)[@bid], sh_gl_heap (sh_hp gs)[@bid] (gl_hp gs)).
 
+Definition as_gheap (h : simple_heap) : heap :=
+  fun x => match x with
+    | SLoc x => None
+    | GLoc x => h x
+  end.
+
+Definition as_sheap (h : simple_heap) : heap :=
+  fun x => match x with
+    | SLoc x => h x
+    | GLoc x => None
+  end.    
+
 Fixpoint safe_ng (n : nat) (gs : g_state nblk ntrd) (Q : assn) :=
   match n with
     | 0 => True
     | S n =>
       ((forall (bid : Fin.t nblk) (tid : Fin.t ntrd), fst ((blks gs)[@bid][@tid]) = SKIP) ->
-         Q default_stack (htop (heap_of_sheap (gl_hp gs)))) /\
+         Q default_stack (htop (as_gheap (gl_hp gs)))) /\
       (forall hF : simple_heap,
          hdisj (gl_hp gs) hF ->
          ~abort_g (Gs (blks gs) (sh_hp gs) (hplus (gl_hp gs) hF))) /\
-      ~ bdiv_g gs /\
+      ~ bdiv_g gs /\ 
       (forall (gs' : g_state nblk ntrd) (hF : simple_heap),
          hdisj (gl_hp gs) hF ->
          red_g (Gs (blks gs) (sh_hp gs) (hplus (gl_hp gs) hF)) gs' ->
@@ -86,27 +98,234 @@ Section For_List_Notation.
       (forall tid bid, snd ks[@bid][@tid] BID = zf bid) ->
       (exists stk,
          (forall tid bid v, v <> TID -> v <> BID -> snd ks[@bid][@tid] v = stk v) /\
-         P stk (htop (heap_of_sheap gh))) ->
+         P stk (htop (as_gheap gh))) ->
     forall n, safe_ng n (Gs ks (const sh nblk) gh) Q.
 
   Definition has_no_vars (P : assn) : Prop := indeP (fun (_ _ : stack) => True) P.
   
   Lemma safe_gl (n : nat) :
-    forall (gs : g_state nblk ntrd) (Q : assn) (Qs : Vector.t assn nblk),
-    (forall bid : Fin.t nblk,
-       safe_nk E n (fst (bs_of_gs gs bid)) (snd (bs_of_gs gs bid)) (sh_spec prog ** Qs[@bid])) ->
-    (forall bid : Fin.t nblk, has_no_vars Qs[@bid]) ->
-    Aistar_v (Qs |= Q) -> 
-    safe_ng n gs Q.
+    forall (gs : g_state nblk ntrd) (ghs : Vector.t heap nblk) (Q : assn) (sh_decl : list (var * nat) )
+           (Qs : Vector.t assn nblk),
+      let sinv := sh_spec sh_decl in
+      disj_eq (Vector.map (@htop loc) ghs) (htop (as_gheap (gl_hp gs))) ->
+      (forall bid : Fin.t nblk,
+         safe_nk E n (fst (bs_of_gs gs bid))
+                 (hplus (as_sheap (sh_hp gs)[@bid]) ghs[@bid]) (sinv ** Qs[@bid])) ->
+      (forall bid : Fin.t nblk, has_no_vars Qs[@bid]) ->
+      Aistar_v Qs |= Q -> 
+      (forall bid tid, sinv (snd (blks gs)[@bid][@tid]) (htop (as_sheap (sh_hp gs)[@bid]))) ->
+      (forall bid tid, inde sinv (writes_var (fst (blks gs)[@bid][@tid]))) ->
+      (forall var, List.In var (List.map fst sh_decl) -> E var = Lo) ->
+      safe_ng n gs Q.
   Proof.
     induction n; simpl; auto.
-    intros gs Q Qs Hsafe Hnov HQ; repeat split.
+    intros gs ghs Q sdec Qs Hdeq Hsafe Hnov HQ Hsinv Hsvar Hslow; repeat split.
     - intros Hskip.
       evar (P : Fin.t nblk -> Prop); assert (Hskipb : forall bid, P bid); [|unfold P in *; clear P].
       { unfold P; intros bid; destruct (Hsafe bid) as (Hskipb & _).
         apply Hskipb in Hskip as (? & ?).
         unfold sat_k in H; simpl in H.
-        lazymatch type of H with (let (_, _) := ?X in _) => destruct X end.
-        unfold has_no_vars, indeP in Hnov; simpl in Hnov; rewrite (Hnov _ _ default_stack) in H; auto.
-        exact H. }
+        lazymatch type of H with (let (_, _) := ?X in _) => destruct X as (srep & Hsrep) end.
+
+        Lemma sh_spec_inde (sdec : list (var * nat)) (stk0 stk1 : stack) (E0 : env) : forall h,
+          (sh_spec sdec) stk0 h -> low_eq E0 stk0 stk1 ->
+          (forall var, List.In var (List.map fst sdec) -> E0 var = Lo) ->
+          (sh_spec sdec) stk1 h.
+        Proof.
+          induction sdec as [|[v n] sdec]; simpl.
+          - intros ? H ? ?; apply H.
+          - intros h H Hlow Hv.
+            destruct H as (ph1 & ph2 & ? & ? & ? & ?); exists ph1, ph2; repeat split; auto.
+            destruct H as [f H]; exists f.
+            clear IHsdec H1 H2; generalize dependent ph1. 
+            generalize 0; induction n; simpl in *; intros st ph1 H; [apply H|].
+            destruct H as (ph1' & ph2' & ? & ? & ? & ?); exists ph1', ph2'; repeat split; auto.
+            unfold low_eq in Hlow; unfold_conn_all; simpl in *; intros x; rewrite <-Hlow; auto.
+        Qed.
+
+        assert ((sh_spec sdec) srep (htop (as_sheap (sh_hp gs)[@bid]))).
+        { assert (exists nt, ntrd = S nt) as [nt Hnt] by (exists (ntrd - 1); omega).
+          generalize dependent gs; rewrite Hnt; intros.
+          apply (sh_spec_inde _ (snd (blks gs)[@bid][@Fin.F1]) _ E); auto.
+          specialize (Hsrep Fin.F1); erewrite nth_map in Hsrep; [apply Hsrep|]; auto. }
+
+        Definition is_sheap (h : heap) := forall x, h (GLoc x) = None.
+        Definition is_gheap (h : heap) := forall x, h (SLoc x) = None.
+        Lemma as_sh_is_sh (h : simple_heap) : is_sheap (as_sheap h).
+        Proof.
+          unfold is_sheap; simpl; auto.
+        Qed.
+        Lemma as_gh_is_gh (h : simple_heap) : is_gheap (as_gheap h).
+        Proof.
+          unfold is_gheap; simpl; auto.
+        Qed.
+
+        Lemma sh_gh_disj (sh gh : heap) : is_sheap sh -> is_gheap gh -> hdisj sh gh.
+        Proof.
+          unfold is_sheap, is_gheap; intros; intros [? | ?]; auto.
+        Qed.
+
+        Lemma htop_hplus (h1 h2 : heap) (H : hdisj h1 h2) :
+          (htop (hplus h1 h2)) = phplus_pheap (proj1 (hdisj_pdisj h1 h2) H).
+        Proof.
+          unfold htop, htop', hplus, phplus_pheap, phplus; simpl; apply pheap_eq.
+          extensionality x; specialize (H x).
+          destruct (h1 x), (h2 x); try auto.
+          destruct H; congruence.
+        Qed.
+
+        Require Import Program.
+        
+        Lemma disj_eq_inj n (hs : Vector.t heap n) :forall h,
+          disj_eq (Vector.map (@htop _) hs) (htop h) ->
+          is_gheap h -> forall i, is_gheap hs[@i].
+        Proof.
+          induction n; simpl; intros h H Hgh i.
+          - inversion i.
+          - dependent destruction hs; dependent destruction i; simpl in *.
+            + intros l.
+              inversion H; subst; simpl; auto.
+              apply (f_equal (fun x => x (SLoc l))) in H4; unfold phplus, htop' in H4.
+              specialize (Hgh l).
+              destruct ph as [ph ?]; simpl in *.
+              destruct (h (SLoc l)), (ph (SLoc l)) as [[? ?]|], (h0 (SLoc l)); congruence.
+            + remember (htop h0) as hh0; inversion H; subst; simpl in *.
+              apply Eqdep.EqdepTheory.inj_pair2 in H3; subst; eauto.
+              apply (f_equal (fun x => this x)) in H2; simpl in H2.
+
+              Lemma htop_phplus_heap (h1 h2 : heap) (ph : pheap) :
+                pdisj (htop h1) ph ->
+                phplus (htop' h1) ph = htop' h2 ->
+                exists ph', ph = htop ph'.
+              Proof.
+                intros;exists (fun x => match PHeap.this ph x with None => None | Some (_,x) => Some x end).
+                destruct ph as [ph ?]; apply pheap_eq.
+                unfold phplus, htop, htop' in *; simpl in *; extensionality x;
+                apply (f_equal (fun f => f x)) in H0.
+                specialize (is_p x); specialize (H x).
+                pose proof frac_contra1.
+                destruct (ph x) as [[? ?]|], (h1 x), (h2 x); first [now auto | congruence | firstorder].
+              Qed.
+
+              pose proof (@htop_phplus_heap _ _ _ hdis H2) as [ht Hht]; subst; auto.
+              eapply IHn.
+              apply H4.
+
+              intros x; apply (f_equal (fun f => f (SLoc x))) in H2; specialize (Hgh x).
+              unfold phplus, htop, htop' in H2; simpl in H2.
+              repeat lazymatch type of H2 with
+                | context [match ?X with | Some _ => _ | None => _ end] => destruct X
+                | context [let (_, _) := ?X in _] => destruct X
+              end; try congruence.
+        Qed.
+
+        assert (hdisj (as_sheap (sh_hp gs)[@bid]) ghs[@bid]).
+        { apply sh_gh_disj; [apply as_sh_is_sh|].
+          apply disj_eq_inj with (as_gheap (gl_hp gs)); auto.
+          apply as_gh_is_gh. }
+        
+        rewrite htop_hplus with (H :=H1) in H.
+
+        Lemma sc_cancel (P Q : assn) s (hp hq : pheap) (Hdis : pdisj hp hq) :
+          precise P ->
+          (P ** Q) s (phplus_pheap Hdis) -> P s hp -> Q s hq.
+        Proof.
+          intros Hprc Hpq Hp; destruct Hpq as (ph1 & ph2 & ? & ? & ? & ?).
+          assert (ph1 = hp).
+          { specialize (Hprc ph1 ph2 hp hq); simpl in Hprc.
+            specialize (Hprc _ H Hp H1 Hdis H2); auto. }
+          assert (ph2 = hq).
+          { subst; simpl in *.
+            apply padd_cancel in H2; auto. }
+          subst; auto.
+        Qed.
+
+        Require Import Qcanon.
+        Lemma precise_ex {T : Type} (P : T -> assn) :
+          (forall s x1 x2 h1 h2, P x1 s h1 -> P x2 s h2 ->
+                                 (forall l q, (exists v0, PHeap.this h1 l = Some (q, v0)) ->
+                                              (exists v1, PHeap.this h2 l = Some (q, v1)))) ->
+          precise (Ex x, P x).
+        Proof.
+          unfold precise; simpl; intros.
+          destruct H0 as [x0 H0], H1 as [x1 H1]; pose proof (H _ _ _ _  _ H0 H1); pose proof (H _ _ _ _ _ H1 H0).
+          destruct h1 as [h1 ?], h1' as [h1' ?]; apply pheap_eq; extensionality l; simpl in *.
+          apply (f_equal (fun f => f l)) in H4;
+            specialize (H2 l); specialize (H3 l); specialize (H5 l); specialize (H6 l).
+          unfold phplus in *; destruct (h1 l) as [[? ?]|], (h1' l) as [[? ?]|],
+            (PHeap.this h2 l) as [[? ?]|], (PHeap.this h2' l) as [[? ?]|]; simpl in *; 
+          try congruence;
+          try (specialize (H5 q); specialize (H6 q);
+               try (destruct H5; [eexists; reflexivity|]; inversion H5; subst);
+               try (destruct H6; [eexists; reflexivity|]; inversion H6; subst);
+               subst; congruence).
+        Qed.
+        
+        Lemma precise_pts e1 q : precise (Ex e2, e1 -->p (q, Enum e2)).
+        Proof.
+          apply precise_ex; intros.
+          unfold_conn_all; rewrite H, H0 in *; destruct H1; eexists;
+          destruct (eq_dec l (ledenot e1 s)); try congruence;
+          inversion H1; reflexivity.
+        Qed.          
+        
+        Lemma precise_ex_star {T : Type} (P Q : T -> assn) :
+          precise ((Ex x, P x) ** (Ex x, Q x)) ->
+          precise (Ex x, P x ** Q x).
+        Proof.
+          unfold precise; simpl; intros.
+          specialize (H h1 h2 h1' h2' s); apply H; auto.
+          destruct H0 as (x & ph1 & ph2 & ? & ? & ? & ?).
+          exists ph1; exists ph2; (repeat split); (try now (exists x; auto)); auto.
+          destruct H1 as (x & ph1 & ph2 & ? & ? & ? & ?).
+          exists ph1; exists ph2; (repeat split); (try now (exists x; auto)); auto.
+        Qed.
+
+        Lemma precise_is_array e n : forall s, precise (Ex f, is_array e n f s).
+        Proof.
+          induction n; simpl; intros.
+          - apply precise_ex; intros; unfold_conn_all.
+            rewrite H, H0 in *; auto.
+          - apply precise_ex_star, precise_star.
+            + apply precise_ex; intros.
+              unfold_conn_all; rewrite H, H0 in *; destruct H1; eexists.
+              destruct (eq_dec l (ledenot _ _)); try congruence;
+              inversion H1; reflexivity.
+            + apply IHn.
+        Qed.
+
+        Lemma precise_sh_spec (sh_dc : list (var * nat)) :
+          precise (sh_spec sh_dc).
+        Proof.
+          induction sh_dc as [|[v n] sh_dc]; simpl; auto.
+          - apply precise_emp.
+          - apply precise_star; auto using precise_is_array.
+        Qed.            
       
+        apply (sc_cancel (sh_spec sdec) Qs[@bid] srep) in H; auto using precise_sh_spec.
+        unfold has_no_vars, indeP in Hnov; simpl in Hnov.
+        rewrite (Hnov _ _ default_stack _) in H; auto.
+        exact H. }
+      simpl in Hskipb.
+      apply HQ.
+
+
+      Lemma aistar_sat {n : nat} : forall (hs : Vector.t pheap n) (h : pheap) (Qs : Vector.t assn n) s ,
+        disj_eq hs h -> (forall i, Qs[@i] s hs[@i]) -> Aistar_v Qs s h.
+      Proof.
+        induction n; dependent destruction hs; dependent destruction Qs; intros.
+        - simpl; inversion H; apply emp_emp_ph.
+        - simpl.
+          inversion H; subst.
+          exists h ph; repeat split; auto.
+          specialize (H0 Fin.F1); apply H0.
+          eapply IHn.
+          apply H5.
+          intros i; specialize (H0 (Fin.FS i)); simpl in H0.
+          apply Eqdep.EqdepTheory.inj_pair2 in H4; subst; auto.
+      Qed.
+
+      eapply aistar_sat; eauto.
+      intros; erewrite Vector.nth_map; [|reflexivity]; auto.
+
+    - 
